src/KV.v
@@ -11,37 +11,6 @@ Require Import Omega.
 
 Set Implicit Arguments.
 
-Lemma addrlen_valulen: addrlen + (valulen - addrlen) = valulen.
-Proof.
-  rewrite valulen_is; auto.
-Qed.
-
-Definition addr2valu (a: addr) : valu.
-  set (zext a (valulen-addrlen)) as r.
-  rewrite addrlen_valulen in r.
-  apply r.
-Defined.
-
-Definition valu2addr (v: valu) : addr.
-  rewrite <- addrlen_valulen in v.
-  apply (split1 addrlen (valulen-addrlen) v).
-Defined.
-
-Lemma addr2valu2addr: forall a,
-  valu2addr (addr2valu a) = a.
-Proof.
-  unfold valu2addr, addr2valu.
-  unfold eq_rec_r, eq_rec.
-  intros.
-  rewrite <- addrlen_valulen.
-  rewrite <- eq_rect_eq_dec; try apply eq_nat_dec.
-  rewrite <- eq_rect_eq_dec; try apply eq_nat_dec.
-  apply split1_combine.
-Qed.
-
-Opaque addr2valu.
-Opaque valu2addr.
-
 Parameter maxlen : addr. (* Number of entries on disk *)
 
 Definition empty_value : valu := $0.
