src/Prog.v
@@ -1,6 +1,7 @@
 Require Import Arith.
 Require Import Word.
 Require Import FunctionalExtensionality.
+Require Import Eqdep_dec.
 
 Set Implicit Arguments.
 
@@ -127,3 +128,34 @@ Proof.
   rewrite upd_ne; auto. rewrite upd_eq; auto. rewrite upd_eq; auto.
   rewrite upd_ne; auto. rewrite upd_ne; auto. rewrite upd_ne; auto. rewrite upd_ne; auto.
 Qed.
+
+Lemma addrlen_valulen: addrlen + (valulen - addrlen) = valulen.
+Proof.
+  rewrite valulen_is; auto.
+Qed.
+
+Definition addr2valu (a: addr) : valu.
+  set (zext a (valulen-addrlen)) as r.
+  rewrite addrlen_valulen in r.
+  apply r.
+Defined.
+
+Definition valu2addr (v: valu) : addr.
+  rewrite <- addrlen_valulen in v.
+  apply (split1 addrlen (valulen-addrlen) v).
+Defined.
+
+Lemma addr2valu2addr: forall a,
+  valu2addr (addr2valu a) = a.
+Proof.
+  unfold valu2addr, addr2valu.
+  unfold eq_rec_r, eq_rec.
+  intros.
+  rewrite <- addrlen_valulen.
+  rewrite <- eq_rect_eq_dec; try apply eq_nat_dec.
+  rewrite <- eq_rect_eq_dec; try apply eq_nat_dec.
+  apply split1_combine.
+Qed.
+
+Opaque addr2valu.
+Opaque valu2addr.
